finish proof of longestPrefix

leetcode/longestPrefix.dfy
@@ -36,104 +36,329 @@ module LongestCommonPrefix {
         if s1 == [] {
             assert s1 + s2 == s2;
         } else {
-            assert s1 == [s1[0]] + s1[1..];
-            ToSetConcat(s1[1..], s2);
             assert [s1[0]]+(s1[1..] + s2) == s1 + s2;
+            ToSetConcat(s1[1..], s2);
         }
     }
+
 
     lemma ToSetHasAll(strs: seq<string>)
         ensures forall x :: x in strs ==> x in ToSet(strs)
     {}
 
-    twostate lemma AllFreshUnionFresh(ss: set<set<Trie>>)
-        requires forall s :: s in ss ==> forall t :: t in s ==> t.Valid()
-        requires forall s :: s in ss ==> fresh(s)
-        ensures fresh(Union(ss))
+    lemma prefixInAllPrefixes(prefix: string, strs: set<string>)
+        requires strs != {}
+        requires IsCommonPrefix(prefix, strs)
+        ensures prefix in AllPrefixes(strs)
     {
 
     }
 
+    ghost function WordsSlice(strs: set<string>): set<string>
+        requires forall s :: s in strs ==> s != ""
+    {
+        if strs == {} then
+            {}
+        else
+            var x :| x in strs;
+            {x[1..]} + WordsSlice(strs - {x})
+    }
+
+    function WordRest(prefix: string, words: set<string>): set<string>
+    {
+        set w | w in words :: prefix + w
+    }
+
+    lemma InWordRest(s: string, prefix: string, suffix: string, words: set<string>)
+        requires s == prefix + suffix
+        requires suffix in words
+        ensures s in WordRest(prefix, words)
+    {
+    }
+
+    lemma WordRestSize(prefix: string, words: set<string>)
+       ensures |WordRest(prefix, words)| == |words|
+    {
+        if words == {} {
+            assert WordRest(prefix, words) == {};
+            assert |WordRest(prefix, words)| == |words|;
+        } else {
+            var x :| x in words;
+            WordRestSize(prefix, words - {x});
+            assert |words| == |words - {x}| + 1;
+            assert |words - {x}| == |WordRest(prefix, words - {x})|;
+            assert WordRest(prefix, words) == WordRest(prefix, words - {x}) + {prefix + x};
+            assert prefix + x !in WordRest(prefix, words - {x}) by {
+                if prefix + x in WordRest(prefix, words - {x}) {
+                    if words - {x} == {} {
+                        assert false;
+                    }
+                    var y :| y in words - {x} && prefix + y == prefix + x;
+                    assert y == (prefix+x)[|prefix|..];
+                    assert y == x;
+                    // assert x in words - {x};
+                    assert false;
+                }
+            }
+            assert prefix + x in WordRest(prefix, words);
+            assert |WordRest(prefix, words)| == |WordRest(prefix, words - {x})| + 1;
+            assert |WordRest(prefix, words)| == |words|;
+        }
+    }
+
+    ghost predicate LongestPrefix(prefix: string, strs: set<string>)
+    {
+        IsCommonPrefix(prefix, strs) && forall prefixes :: prefixes in AllPrefixes(strs) && IsCommonPrefix(prefixes, strs) ==> |prefixes| <= |prefix|
+    }
+
+    lemma LongestPredicateUnique(prefixA: string, prefixB: string, strs: set<string>)
+        requires strs != {}
+        requires LongestPrefix(prefixA, strs)
+        requires LongestPrefix(prefixB, strs)
+        ensures prefixA == prefixB
+    {}
 
 
-    // twostate predicate UnionFresh(t: Trie)
-    //     requires t.Valid()
-    //     requires forall k :: k in t.children.Keys ==> fresh(t.children[k].repr)
-    // {
-    //    fresh(Union(set k | k in t.children.Keys :: t.children[k].repr)) 
-    // }
 
-    method {:vcs_split_on_every_assert} longestCommonPrefix(strs: seq<string>) returns (prefix: string)
+
+    lemma shortestWordsIsLongestedPrefix(strs: set<string>, short: string, long: string)
+        requires short in strs
+        requires long in strs
+        requires |long| > |short|
+        requires IsCommonPrefix(short, strs)
+        ensures !IsCommonPrefix(long, strs)
+    {}
+
+    lemma longestPrefixIsShortestWord(strs: set<string>, short: string)
+        requires short in strs
+        requires IsCommonPrefix(short, strs)
+        ensures LongestPrefix(short, strs)
+    {}
+
+    lemma WordRestChild(t: Trie, key: char)
+        requires t.Valid()
+        requires key in t.children.Keys
+        ensures WordRest([key], t.children[key].words) == set w | w in t.words && |w| > 0 && w[0] == key
+    {
+        var keyWords := set w | w in t.words && |w| > 0 && w[0] == key;
+        WordRestSize([key], t.children[key].words);
+        if t.children[key].words == {} {
+            assert key in t.firstChars;
+            var w :| w in t.words && |w| > 0 && w[0] == key;
+            assert w in t.words;
+            assert w in keyWords;
+            assert w[1..] in t.children[key].words;
+            assert false;
+        } else {
+            forall kw | kw in keyWords
+                ensures kw in WordRest([key], t.children[key].words)
+            {
+                assert kw in t.words;
+                assert kw[0] == key;
+                assert kw[1..] in t.children[key].words;
+                assert kw == [key] + kw[1..];
+                assert kw in WordRest([key], t.children[key].words);
+            }
+
+            forall w | w in WordRest([key], t.children[key].words)
+                ensures w in keyWords
+            {
+                var tw :| tw in t.children[key].words && [key] + tw == w;
+                assert tw in t.children[key].words;
+                assert |w| > 0;
+                assert w[0] == key;
+                forall kw | kw in t.words && |kw| > 0 && kw[0] == key && kw != w
+                    ensures kw[1..] != tw
+                {
+                }
+                assert w in t.words by {
+                    if w !in t.words {
+                        assert tw == w[1..];
+                        assert tw !in t.children[key].words;
+                        assert false;
+                    }
+                }
+            }
+        }
+    }
+
+            // invariant trie.words != {} ==> trie.children.Keys != {}
+            // invariant fresh(trie)
+            // invariant fresh(trie.repr)
+            // invariant forall k :: k in trie.children.Keys ==> fresh(trie.children[k]) && fresh(trie.children[k].repr)
+            // invariant trie.children.Keys == {} ==> fresh(trie.repr)
+            // invariant trie.children.Keys != {} ==> fresh(trie.repr)
+            // invariant fresh(Union(set k | k in trie.children.Keys :: trie.children[k].repr)) /// <<EXPLODES!
+            // invariant fresh(Union(trie.ReprSet()))
+            // invariant fresh(trie.repr-old@Begin(trie.repr))
+    lemma  {:vcs_split_on_every_assert} longestPrefixOfTrieWithMultipleKeys(t: Trie, prefix: string, words: set<string>)
+        requires t.children.Keys != {}
+        requires |t.children.Keys| > 1
+        requires "" !in t.words
+        requires t.Valid()
+        requires words == WordRest(prefix, t.words)
+        requires IsCommonPrefix(prefix, words)
+        ensures LongestPrefix(prefix, words)
+    {
+
+        if longerPrefix :| longerPrefix in AllPrefixes(words) && IsCommonPrefix(longerPrefix, words) && |longerPrefix| > |prefix| {
+            var c := longerPrefix[|prefix|];
+            // assert c in t.children.Keys;
+            assert t.children.Keys-{c} != {} by {
+                if (t.children.Keys-{c}) == {} {
+                    assert (t.children.Keys-{c})+{c} == {} + {c};
+                    assert t.children.Keys == {c};
+                    assert |t.children.Keys| == 1;
+                    assert false;
+                }
+            }
+            var b :| b in t.children.Keys && b != c;
+            var bword :| bword in t.words && bword[0] == b && |bword| > 0;
+            assert bword == [b] + bword[1..];
+            var bwords := WordRest(prefix+[b], t.children[b].words);
+            assert t.children[b].words == set w | w in t.words && w[0]==b :: w[1..];
+            InWordRest(prefix + bword, prefix+[b], bword[1..], t.children[b].words);
+            
+            // assert  bwords != {};
+            assert bwords < words by {
+                forall w | w in bwords
+                    ensures w in words
+                {
+                    var tw :| tw in t.children[b].words && prefix+[b] + tw == w;
+                    var bw := [b] + tw;
+                    var bs := set bw | bw in t.words && |bw| > 0 && bw[0] == b;
+                    WordRestChild(t, b);
+                    assert bs == WordRest([b], t.children[b].words);
+                    assert bw in bs by {
+                        if bw !in bs {
+                            assert bw[0] == b;
+                            assert bw[1..] !in t.children[b].words;
+                            assert false;
+                        }
+                    }
+                    assert prefix + bw == w;
+                }
+            }
+            assert false;
+        }
+    }
+
+    method longestCommonPrefix(strs: seq<string>) returns (prefix: string)
         requires strs != []
-        requires forall i :: 0 <= i < |strs| ==> strs[i] != ""
-        ensures IsCommonPrefix(prefix, ToSet(strs))
-        ensures forall prefixes :: prefixes in AllPrefixes(ToSet(strs)) ==> |prefixes| <= |prefix|
+        ensures LongestPrefix(prefix, ToSet(strs))
     {
         var trie := new Trie();
-        assert fresh(trie.repr);
-        assert trie.Valid();
-        assert fresh(trie);
         label Begin:
         for i := 0 to |strs| 
             invariant allocated(trie)
-            invariant "" !in strs[0..i]
-            // invariant trie.words != {} ==> trie.children.Keys != {}
-            invariant fresh(trie)
-            invariant fresh(trie.repr)
-            invariant forall k :: k in trie.children.Keys ==> fresh(trie.children[k]) && fresh(trie.children[k].repr)
-            invariant trie.children.Keys == {} ==> fresh(trie.repr)
-            invariant trie.children.Keys != {} ==> fresh(trie.repr)
-            // invariant fresh(Union(set k | k in trie.children.Keys :: trie.children[k].repr)) /// <<EXPLODES!
-            invariant fresh(Union(trie.ReprSet()))
-            // invariant fresh(trie.repr-old@Begin(trie.repr))
+            invariant fresh(trie.repr - old@Begin(trie.repr))
             invariant 0 <= i <= |strs|
             invariant trie.Valid()
             invariant trie.words == ToSet(strs[0..i])
-            modifies  trie, trie.repr
         {
-            assert strs == strs[0..i] + strs[i..];
-            // label PreInsert:
-            if trie.children.Keys == {} {
-                // assert "" !in trie.words;
-                // assert trie.words == {};
-            } else {
-                UnionHasAll(set k | k in trie.children.Keys :: trie.children[k].repr);
-                NotInAllNotInUnion(set k | k in trie.children.Keys :: trie.children[k].repr, trie);
-                assert trie !in Union(set k | k in trie.children.Keys :: trie.children[k].repr);
-                assert trie.repr == {trie} + Union(set k | k in trie.children.Keys :: trie.children[k].repr);
-                assert Union(set k | k in trie.children.Keys :: trie.children[k].repr) < trie.repr;
-                ghost var foo := set key | key in trie.children.Keys :: trie.children[key].repr;
-                // assert foo == ReprSet(trie);
-
-                // AllFreshUnionFresh(trie.ReprSet());
-                // assert fresh(Union(set k | k in trie.children.Keys :: trie.children[k].repr));
-                // assert trie.words == Union(set k | k in trie.children.Keys :: trie.children[k].repr);
-            }
             trie.insertRecursive(strs[i]);
             assert strs[0..i+1] == strs[0..i] + [strs[i]];
             ToSetConcat(strs[0..i], [strs[i]]);
-            ToSetHasAll(strs[0..i+1]);
-            // assert trie.words == old@PreInsert(trie.words) + {strs[i]};
         }
         assert strs == strs[0..|strs|];
         assert ToSet(strs) == ToSet(strs[0..|strs|]);
         assert ToSet(strs) == trie.words;
-        prefix := longestCommonPrefixRec(trie, "");
+        assert WordRest("", ToSet(strs)) == ToSet(strs) by {
+            forall w | w in ToSet(strs)
+                ensures "" + w in ToSet(strs)
+            {
+                assert "" + w == w;
+            }
+
+            forall w | w in ToSet(strs)
+                ensures w in WordRest("", ToSet(strs))
+            {
+                assert "" + w == w;
+                assert w in WordRest("", ToSet(strs));
+            }
+        }
+        prefix := longestCommonPrefixRec(trie, "", trie.words);
     }
 
-    method {:verify false} longestCommonPrefixRec(t: Trie, prefix: string) returns (prefix': string)
+    method longestCommonPrefixRec(t: Trie, prefix: string, ghost words: set<string>) returns (prefix': string)
+        requires words != {}
         requires t.Valid()
-        requires IsCommonPrefix(prefix, t.words)
-        ensures IsCommonPrefix(prefix', t.words)
-        ensures forall prefixes :: prefixes in AllPrefixes(t.words) ==> |prefixes| <= |prefix|
+        requires t.words == words
+        requires WordRest(prefix, t.words) != {}
+        requires IsCommonPrefix(prefix, WordRest(prefix, t.words))
+        ensures IsCommonPrefix(prefix', WordRest(prefix, t.words))
+        decreases t.repr
+        ensures LongestPrefix(prefix', WordRest(prefix, words))
     {
         if |t.children.Keys| == 1 {
             if t.isWord {
+                assert "" in t.words;
+                assert prefix + "" == prefix;
+                assert prefix + "" in WordRest(prefix, t.words);
+                assert prefix in WordRest(prefix, t.words);
+                longestPrefixIsShortestWord(WordRest(prefix, t.words), prefix);
                 return prefix;
             }else{
                 var key :| key in t.children.Keys;
-                prefix' := longestCommonPrefixRec(t.children[key], prefix + [key]);
+                forall w | w in t.words 
+                    ensures w[0] == key
+                {
+                    if w[0] != key {
+                        assert w[0] in t.children.Keys;
+                        assert |t.children.Keys-{key}| == 0;
+                        assert false;
+                    }
+                }
+                assert t.children[key].words == set w | w in t.words :: w[1..];
+                assert WordRest(prefix+[key], t.children[key].words) == WordRest(prefix, t.words) by {
+                    forall w | w in t.children[key].words
+                        ensures prefix + [key] + w in WordRest(prefix, t.words)
+                    {
+                        assert w in (set tw | tw in t.words :: tw[1..]);
+                        var tw :| tw in t.words && tw[1..] == w;
+                        assert tw in t.words;
+                        assert tw == [key] + w;
+                        assert prefix + tw in WordRest(prefix, t.words);
+                        assert prefix + tw == prefix + [key] + w;
+                        assert prefix +[key] + w in WordRest(prefix, t.words);
+                    }
+                    forall w | w in WordRest(prefix, t.words)
+                        ensures w in WordRest(prefix+[key], t.children[key].words)
+                    {
+                        var tw :| tw in t.words && prefix + tw == w;
+                        assert tw[0] == key;
+                        assert tw[1..] in t.children[key].words;
+                        assert prefix +[key] + tw[1..] == w;
+                        assert w in WordRest(prefix+[key], t.children[key].words);
+                    }
+                }
+                assert t.children[key].words != {};
+                prefix' := longestCommonPrefixRec(t.children[key], prefix + [key], t.children[key].words);
                 return prefix';
+            }
+        }
+        if |t.children.Keys| == 0 {
+            assert t.children.Keys == {};
+            assert t.words <= {""} by {
+                if w :| w in t.words && w != "" {
+                    assert w in t.words;
+                    assert w[0] in t.children.Keys;
+                    assert false;
+                }
+            }
+            assert t.words != {};
+            assert t.words == {""};
+            assert prefix + "" == prefix;
+            assert prefix in WordRest(prefix, t.words);
+            longestPrefixIsShortestWord(WordRest(prefix, t.words), prefix);
+            
+        }else{
+            if "" in t.words {
+                assert prefix + "" == prefix;
+                assert prefix in WordRest(prefix, t.words);
+                longestPrefixIsShortestWord(WordRest(prefix, t.words), prefix);
+            }else{
+                longestPrefixOfTrieWithMultipleKeys(t, prefix, WordRest(prefix, words));
             }
         }
         return prefix;
